more integration

src/Horizontal.ec
@@ -16,17 +16,11 @@ clone import Language as L.
 clone import MultiPartyProtocolAPISemantics as Source with
  type L1.L = L,
  type L2.L = L,
- type L3.L = L.
-
-clone import Language as L1'.
-clone import Language as L2'.
-clone import Language as L3'.
-
-clone import MultiPartyProtocolAPISemantics as Target with
-  type L1.L = L1'.L,
-  type L2.L = L2'.L,
-  type L3.L = L3'.L.
-import MultiPartyAPISemantics.
+ type L3.L = L,
+  type MultiPartyAPISemantics.SemP2.EnvL = MultiPartyAPISemantics.SemP1.EnvL,
+  type MultiPartyAPISemantics.SemP3.EnvL = MultiPartyAPISemantics.SemP1.EnvL,
+  op MultiPartyAPISemantics.SemP2.stepL = MultiPartyAPISemantics.SemP1.stepL,
+  op MultiPartyAPISemantics.SemP3.stepL = MultiPartyAPISemantics.SemP1.stepL.
 
 (* The REAL API *)
 module API_Real : API.API_t = {
@@ -71,6 +65,7 @@ proc sop(sop: MPCLib.sop_t, pargs: value_t list, sargs: svar_t list, a : svar_t)
 }
 }.
 
+import MultiPartyAPISemantics.
 import MultiPartySemantics.
 
 lemma nosmt stepP_spec_h i st':
@@ -180,6 +175,17 @@ lemma nosmt stepP_spec i st':
          ] = 1%r.
 proof. by conseq stepP_ll (stepP_spec_h i st'). qed.
 
+clone import Language as L1'.
+clone import Language as L2'.
+clone import Language as L3'.
+
+clone import MultiPartyProtocolAPISemantics as Target with
+  type L1.L = L1'.L,
+  type L2.L = L2'.L,
+  type L3.L = L3'.L.
+import MultiPartyAPISemantics.
+import MultiPartySemantics.
+
 (** COMPILERS **)
 
 (* Compiler Correctness *)
@@ -254,17 +260,26 @@ axiom bisim_backward3 ss st kt st':
                  /\ equivSt3 ss' st' /\ 0 <= ks).
 
 (* handling different paces among parties *)
-op advSt1 ['l,'e] step (ss: (L,Source.MultiPartyAPISemantics.SemP1.EnvL) Source.MultiPartyAPISemantics.SemP1.APIst) (st: ('l,'e) Target.MultiPartyAPISemantics.SemP1.APIst) : bool =
+print Target.MultiPartyAPISemantics.SemP1.stepL.
+
+op advSt1
+(step : L1.L -> Target.MultiPartyAPISemantics.SemP1.EnvL -> Target.MultiPartyAPISemantics.SemP1.API.apiRes_data option -> (L1.L, Target.MultiPartyAPISemantics.SemP1.EnvL) Target.MultiPartyAPISemantics.SemP1.ECall option)
+(ss: (L.L, Source.MultiPartyAPISemantics.SemP1.EnvL) Source.MultiPartyAPISemantics.SemP1.APIst) 
+(st: (L1.L, Target.MultiPartyAPISemantics.SemP1.EnvL) Target.MultiPartyAPISemantics.SemP1.APIst) : bool =
  exists n st', 0 <= n /\ equivSt1 ss st' /\ Target.MultiPartyAPISemantics.SemP1.stepPiter step n st' = Some st.
 
-lemma advS01 ['l, 'e] step s1 (s2: ('l, 'e) Target.MultiPartyAPISemantics.SemP1.APIst):
+lemma advS01 (step : L1.L -> Target.MultiPartyAPISemantics.SemP1.EnvL -> Target.MultiPartyAPISemantics.SemP1.API.apiRes_data option -> (L1.L, Target.MultiPartyAPISemantics.SemP1.EnvL) Target.MultiPartyAPISemantics.SemP1.ECall option) 
+(s1 :  (L.L, Source.MultiPartyAPISemantics.SemP1.EnvL) Source.MultiPartyAPISemantics.SemP1.APIst)
+(s2: (L1.L, Target.MultiPartyAPISemantics.SemP1.EnvL) Target.MultiPartyAPISemantics.SemP1.APIst):
  equivSt1 s1 s2 => advSt1 step s1 s2.
 proof.
 move=> *; exists 0 s2; progress.
 by rewrite Target.MultiPartyAPISemantics.SemP1.stepPiter0.
 qed.
 
-lemma nosmt advSt_callSt1 ['l, 'e] step s1 (s2: ('l, 'e) Target.MultiPartyAPISemantics.SemP1.APIst):
+lemma nosmt advSt_callSt1 (step : L1.L -> Target.MultiPartyAPISemantics.SemP1.EnvL -> Target.MultiPartyAPISemantics.SemP1.API.apiRes_data option -> (L1.L, Target.MultiPartyAPISemantics.SemP1.EnvL) Target.MultiPartyAPISemantics.SemP1.ECall option) 
+(s1 :  (L.L, Source.MultiPartyAPISemantics.SemP1.EnvL) Source.MultiPartyAPISemantics.SemP1.APIst)
+(s2: (L1.L, Target.MultiPartyAPISemantics.SemP1.EnvL) Target.MultiPartyAPISemantics.SemP1.APIst):
  advSt1 step s1 s2 =>
  Target.MultiPartyAPISemantics.SemP1.callSt s1 <> None =>
  equivSt1 s1 s2.
@@ -276,17 +291,24 @@ move: (Target.MultiPartyAPISemantics.SemP1.callSt_stepPiter step k st' H4); move
 by move: H2; rewrite H5.
 qed.
 
-op advSt2 ['l,'e] step (ss: (L,Source.MultiPartyAPISemantics.SemP2.EnvL) Source.MultiPartyAPISemantics.SemP2.APIst) (st: ('l,'e) Target.MultiPartyAPISemantics.SemP2.APIst) : bool =
+op advSt2
+(step : L2.L -> Target.MultiPartyAPISemantics.SemP2.EnvL -> Target.MultiPartyAPISemantics.SemP2.API.apiRes_data option -> (L2.L, Target.MultiPartyAPISemantics.SemP2.EnvL) Target.MultiPartyAPISemantics.SemP2.ECall option)
+(ss: (L.L, Source.MultiPartyAPISemantics.SemP2.EnvL) Source.MultiPartyAPISemantics.SemP2.APIst) 
+(st: (L2.L, Target.MultiPartyAPISemantics.SemP2.EnvL) Target.MultiPartyAPISemantics.SemP2.APIst) : bool =
  exists n st', 0 <= n /\ equivSt2 ss st' /\ Target.MultiPartyAPISemantics.SemP2.stepPiter step n st' = Some st.
 
-lemma advS02 ['l, 'e] step s1 (s2: ('l, 'e) Target.MultiPartyAPISemantics.SemP2.APIst):
- equivSt1 s1 s2 => advSt1 step s1 s2.
+lemma advS02 (step : L2.L -> Target.MultiPartyAPISemantics.SemP2.EnvL -> Target.MultiPartyAPISemantics.SemP2.API.apiRes_data option -> (L2.L, Target.MultiPartyAPISemantics.SemP2.EnvL) Target.MultiPartyAPISemantics.SemP2.ECall option) 
+(s1 :  (L.L, Source.MultiPartyAPISemantics.SemP2.EnvL) Source.MultiPartyAPISemantics.SemP2.APIst)
+(s2: (L2.L, Target.MultiPartyAPISemantics.SemP2.EnvL) Target.MultiPartyAPISemantics.SemP2.APIst):
+ equivSt2 s1 s2 => advSt2 step s1 s2.
 proof.
 move=> *; exists 0 s2; progress.
 by rewrite Target.MultiPartyAPISemantics.SemP2.stepPiter0.
 qed.
 
-lemma nosmt advSt_callSt2 ['l, 'e] step s1 (s2: ('l, 'e) Target.MultiPartyAPISemantics.SemP2.APIst):
+lemma nosmt advSt_callSt2 (step : L2.L -> Target.MultiPartyAPISemantics.SemP2.EnvL -> Target.MultiPartyAPISemantics.SemP2.API.apiRes_data option -> (L2.L, Target.MultiPartyAPISemantics.SemP2.EnvL) Target.MultiPartyAPISemantics.SemP2.ECall option) 
+(s1 :  (L.L, Source.MultiPartyAPISemantics.SemP2.EnvL) Source.MultiPartyAPISemantics.SemP2.APIst)
+(s2: (L2.L, Target.MultiPartyAPISemantics.SemP2.EnvL) Target.MultiPartyAPISemantics.SemP2.APIst):
  advSt2 step s1 s2 =>
  Target.MultiPartyAPISemantics.SemP2.callSt s1 <> None =>
  equivSt2 s1 s2.
@@ -298,17 +320,24 @@ move: (Target.MultiPartyAPISemantics.SemP2.callSt_stepPiter step k st' H4); move
 by move: H2; rewrite H5.
 qed.
 
-op advSt3 ['l,'e] step (ss: (L,Source.MultiPartyAPISemantics.SemP3.EnvL) Source.MultiPartyAPISemantics.SemP3.APIst) (st: ('l,'e) Target.MultiPartyAPISemantics.SemP3.APIst) : bool =
+op advSt3
+(step : L3.L -> Target.MultiPartyAPISemantics.SemP3.EnvL -> Target.MultiPartyAPISemantics.SemP3.API.apiRes_data option -> (L3.L, Target.MultiPartyAPISemantics.SemP3.EnvL) Target.MultiPartyAPISemantics.SemP3.ECall option)
+(ss: (L.L, Source.MultiPartyAPISemantics.SemP3.EnvL) Source.MultiPartyAPISemantics.SemP3.APIst) 
+(st: (L3.L, Target.MultiPartyAPISemantics.SemP3.EnvL) Target.MultiPartyAPISemantics.SemP3.APIst) : bool =
  exists n st', 0 <= n /\ equivSt3 ss st' /\ Target.MultiPartyAPISemantics.SemP3.stepPiter step n st' = Some st.
 
-lemma advS03 ['l, 'e] step s1 (s2: ('l, 'e) Target.MultiPartyAPISemantics.SemP3.APIst):
+lemma advS03 (step : L3.L -> Target.MultiPartyAPISemantics.SemP3.EnvL -> Target.MultiPartyAPISemantics.SemP3.API.apiRes_data option -> (L3.L, Target.MultiPartyAPISemantics.SemP3.EnvL) Target.MultiPartyAPISemantics.SemP3.ECall option) 
+(s1 :  (L.L, Source.MultiPartyAPISemantics.SemP3.EnvL) Source.MultiPartyAPISemantics.SemP3.APIst)
+(s2: (L3.L, Target.MultiPartyAPISemantics.SemP3.EnvL) Target.MultiPartyAPISemantics.SemP3.APIst):
  equivSt3 s1 s2 => advSt3 step s1 s2.
 proof.
 move=> *; exists 0 s2; progress.
 by rewrite Target.MultiPartyAPISemantics.SemP3.stepPiter0.
 qed.
 
-lemma nosmt advSt_callSt3 ['l, 'e] step s1 (s2: ('l, 'e) Target.MultiPartyAPISemantics.SemP3.APIst):
+lemma nosmt advSt_callSt3 (step : L3.L -> Target.MultiPartyAPISemantics.SemP3.EnvL -> Target.MultiPartyAPISemantics.SemP3.API.apiRes_data option -> (L3.L, Target.MultiPartyAPISemantics.SemP3.EnvL) Target.MultiPartyAPISemantics.SemP3.ECall option) 
+(s1 :  (L.L, Source.MultiPartyAPISemantics.SemP3.EnvL) Source.MultiPartyAPISemantics.SemP3.APIst)
+(s2: (L3.L, Target.MultiPartyAPISemantics.SemP3.EnvL) Target.MultiPartyAPISemantics.SemP3.APIst):
  advSt3 step s1 s2 =>
  Target.MultiPartyAPISemantics.SemP3.callSt s1 <> None =>
  equivSt3 s1 s2.
@@ -319,13 +348,13 @@ move: (Target.MultiPartyAPISemantics.SemP3.callSt_stepPiter step k st' H4); move
  by move: H2; rewrite Target.MultiPartyAPISemantics.SemP3.stepPiter0 //.
 by move: H2; rewrite H5.
 qed.
-
 (*module RealSemMT: RealSemInterface = {
   module PSem = ProgSemMT(API_Real)
   include PSem
 }.*)
 
 module RealSemMT = Target.ProgSem(API_Real).
+module RealSem = Source.ProgSem(API_Real).
 
 module AdvOrclMT (Sem: AdvSemInterface) : AdvSemInterface = {
   (* Simulator runs a local copy of all parties... *)
@@ -382,125 +411,217 @@ section MTSecurityProof.
 declare module A: Adversary{ProgSem, ProgSem, AdvOrclMT}.
 declare module Z: Environment{A, API_Real, ProgSem, AdvOrclMT}.
 
-op inv (stMT1 stMT2: GlobalMTSt) (stST2: GlobalSt) =
- stMT2.`P1 = stMT1.`P1 /\
- stMT2.`P2 = stMT1.`P2 /\
- stMT2.`P3 = stMT1.`P3 /\
- stST2.`ib = stMT1.`ibmt /\
- stST2.`ob = stMT1.`obmt /\
- stST2.`Sigma.[1] <> None /\
- stST2.`Sigma.[2] = stST2.`Sigma.[1] /\
- stST2.`Sigma.[3] = stST2.`Sigma.[1] /\
- advSt stepL1 (oget stST2.`Sigma.[1]) stMT1.`P1 /\
- advSt stepL2 (oget stST2.`Sigma.[1]) stMT1.`P2 /\
- advSt stepL3 (oget stST2.`Sigma.[1]) stMT1.`P3.
+op inv (stMT1 stMT2: Target.MultiPartyAPISemantics.GlobalSt) (stST2: Source.MultiPartyAPISemantics.GlobalSt) =
+ stMT2.`StP1 = stMT1.`StP1 /\
+ stMT2.`StP2 = stMT1.`StP2 /\
+ stMT2.`StP3 = stMT1.`StP3 /\
+ Source.MultiPartyAPISemantics.ib stST2 = stMT1.`ib /\
+ Source.MultiPartyAPISemantics.ob stST2 = stMT1.`ob /\
+ Source.MultiPartyAPISemantics.StP1 stST2 = Source.MultiPartyAPISemantics.StP2 stST2 /\
+  Source.MultiPartyAPISemantics.StP2 stST2 = Source.MultiPartyAPISemantics.StP3 stST2 /\
+ advSt1 Target.MultiPartyAPISemantics.SemP1.stepL (Source.MultiPartyAPISemantics.StP1 stST2) stMT1.`StP1 /\
+ advSt2 Target.MultiPartyAPISemantics.SemP2.stepL (Source.MultiPartyAPISemantics.StP2 stST2) stMT1.`StP2 /\
+ advSt3 Target.MultiPartyAPISemantics.SemP3.stepL (Source.MultiPartyAPISemantics.StP3 stST2) stMT1.`StP3.
 
 local lemma nosmt stepP_prop:
  equiv [ RealSemMT.stepP ~ AdvOrclMT(RealSem).stepP:
          ={id} /\ ={API_Real.senv} /\
-         inv ProgSemMT.st{1} ProgSemMT.st{2} ProgSem.st{2}
+         inv Target.ProgSem.st{1} Target.ProgSem.st{2} Source.ProgSem.st{2}
          ==>
          ={res} /\ ={API_Real.senv} /\
-         inv ProgSemMT.st{1} ProgSemMT.st{2} ProgSem.st{2} ].
+         inv Target.ProgSem.st{1} Target.ProgSem.st{2} Source.ProgSem.st{2} ].
 proof.
-proc; wp; skip; rewrite /inv; progress.
+proc.
+sp.
+match => //=.
+if => //=.
+smt().
+sp 1 1.
+if => //=.
+smt().
+wp; skip; rewrite /inv; progress.
+- smt(). smt(). smt(). smt(). smt(). smt(). smt().
+- move: H6 => [??[?[??]]].
+exists (n+1) st'; progress; rewrite /upd_Sigma1 /=; first smt().
+  apply: (Target.MultiPartyAPISemantics.SemP1.stepPiterS_some _ _ _ _ _ _ H12) => //=.
+  by rewrite -some_oget //.
+smt(). smt().
+
+if => //=.
+smt().
+sp 1 1.
+if => //=.
+smt().
+wp; skip; rewrite /inv; progress.
 - smt(). smt(). smt(). smt(). smt(). smt(). smt(). smt().
 - move: H7 => [??[?[??]]].
-  exists (n+1) st'; progress; rewrite /upd_P1 /=; first smt().
-  apply: (stepPiterS_some _ _ _ _ _ _ H15) => //=.
+exists (n+1) st'; progress; rewrite /upd_Sigma2 /=; first smt().
+  apply: (Target.MultiPartyAPISemantics.SemP2.stepPiterS_some _ _ _ _ _ _ H12) => //=.
   by rewrite -some_oget //.
-- smt(). smt(). smt(). smt(). smt(). smt(). smt(). smt().
-  smt(). smt(). smt().
+smt(). 
+
+if => //=.
+smt().
+sp 1 1.
+if => //=.
+smt().
+wp; skip; rewrite /inv; progress.
+- smt(). smt(). smt(). smt(). smt(). smt(). smt(). smt(). smt().
 - move: H8 => [??[?[??]]].
-  exists (n+1) st'; progress; rewrite /upd_P2 /=; first smt().
-  apply: (stepPiterS_some _ _ _ _ _ _ H16) => //=.
+exists (n+1) st'; progress; rewrite /upd_Sigma3 /=; first smt().
+  apply: (Target.MultiPartyAPISemantics.SemP3.stepPiterS_some _ _ _ _ _ _ H12) => //=.
   by rewrite -some_oget //.
-- smt(). smt(). smt(). smt(). smt(). smt(). smt(). smt().
-  smt(). smt(). smt().
-- move: H9 => [??[?[??]]].
-  exists (n+1) st'; progress; rewrite /upd_P3 /=; first smt().
-  apply: (stepPiterS_some _ _ _ _ _ _ H17) => //=.
-  by rewrite -some_oget //.
-- smt(). smt(). smt().
+qed.
+
+lemma local_source_step12 : Source.MultiPartyAPISemantics.SemP1.stepL = Source.MultiPartyAPISemantics.SemP2.stepL.
+proof.
+rewrite fun_ext /(==) => ? /#.
 qed.
 
 local lemma nosmt stepS_prop:
  equiv [ RealSemMT.stepS ~ AdvOrclMT(RealSem).stepS:
          true /\ ={API_Real.senv} /\
-         inv ProgSemMT.st{1} ProgSemMT.st{2} ProgSem.st{2}
+         inv Target.ProgSem.st{1} Target.ProgSem.st{2} Source.ProgSem.st{2}
          ==>
          ={res} /\ ={API_Real.senv} /\
-         inv ProgSemMT.st{1} ProgSemMT.st{2} ProgSem.st{2} ].
+         inv Target.ProgSem.st{1} Target.ProgSem.st{2} Source.ProgSem.st{2} ].
 proof.
 proc.
 sp 2 2; simplify.
 if; [smt() | | by skip; progress].
-seq 0 0: ((exists ks ss',
-            stepPiter stepL ks (oget ProgSem.st{2}.`Sigma.[1])
+seq 0 0: ((exists (ks : int) ss',
+            (*stepPiter stepL ks (oget ProgSem.st{2}.`Sigma.[1])*)
+            Source.MultiPartyAPISemantics.SemP1.stepPiter Source.MultiPartyAPISemantics.SemP1.stepL ks (Source.MultiPartyAPISemantics.StP1 Source.ProgSem.st{2})
             = Some ss' /\
-            equivSt ss' ProgSemMT.st{1}.`P1 /\ 0 <= ks)
+            equivSt1 ss' Target.ProgSem.st{1}.`StP1 /\ 0 <= ks)
           /\ #[/:]pre).
  skip; rewrite /inv => |> *.
- move: H7 => [??[?[??]]].
- apply (bisim_backward1 _ _ _ _ H11 H12 _); smt(). 
+ move: H6 => [??[?[??]]].
+ apply (bisim_backward1 _ _ _ _ H10 H11 _); smt(). 
 elim* => ??.
-exists* (oget ProgSem.st{2}.`Sigma.[1]); elim* => ss.
-conseq (_: ss = oget ProgSem.st{2}.`Sigma.[1] /\
-           stepPiter stepL ks ss = Some ss' /\
-           equivSt ss' ProgSemMT.st{1}.`P1 /\
-           equivSt ss' ProgSemMT.st{1}.`P2 /\
-           equivSt ss' ProgSemMT.st{1}.`P3 /\
+exists* (Source.MultiPartyAPISemantics.StP1 Source.ProgSem.st{2}); elim* => ss.
+conseq (_: ss = Source.MultiPartyAPISemantics.StP1 Source.ProgSem.st{2} /\
+           Source.MultiPartyAPISemantics.SemP1.stepPiter Source.MultiPartyAPISemantics.SemP1.stepL ks (Source.MultiPartyAPISemantics.StP1 Source.ProgSem.st{2}) = Some ss' /\
+           equivSt1 ss' Target.ProgSem.st{1}.`StP1 /\
+           equivSt2 ss' Target.ProgSem.st{1}.`StP2 /\
+           equivSt3 ss' Target.ProgSem.st{1}.`StP3 /\
            ={r,ecall,API_Real.senv} /\
            0 <= ks /\ r{2}=None /\
-           ecall{2} = callSt ProgSemMT.st{2}.`P1 /\
-           ecall{2} = callSt ProgSemMT.st{2}.`P2 /\
-           ecall{2} = callSt ProgSemMT.st{2}.`P3 /\
+           ecall{2} = Target.MultiPartyAPISemantics.SemP1.callSt Target.ProgSem.st{2}.`StP1 /\
+           ecall{2} = Target.MultiPartyAPISemantics.SemP2.callSt Target.ProgSem.st{2}.`StP2 /\
+           ecall{2} = Target.MultiPartyAPISemantics.SemP3.callSt Target.ProgSem.st{2}.`StP3 /\
            ecall{2} <> None /\
-           ProgSemMT.st{2}.`P1 = ProgSemMT.st{1}.`P1 /\
-           ProgSemMT.st{2}.`P2 = ProgSemMT.st{1}.`P2 /\
-           ProgSemMT.st{2}.`P3 = ProgSemMT.st{1}.`P3 /\
-           ProgSem.st{2}.`ib = ProgSemMT.st{1}.`ibmt /\
-           ProgSem.st{2}.`ob = ProgSemMT.st{1}.`obmt /\
-           ProgSem.st{2}.`Sigma.[1] <> None /\
-           ProgSem.st{2}.`Sigma.[2] = ProgSem.st{2}.`Sigma.[1] /\
-           ProgSem.st{2}.`Sigma.[3] = ProgSem.st{2}.`Sigma.[1]
+           Target.ProgSem.st{2}.`StP1 = Target.ProgSem.st{1}.`StP1 /\
+           Target.ProgSem.st{2}.`StP2 = Target.ProgSem.st{1}.`StP2 /\
+           Target.ProgSem.st{2}.`StP3 = Target.ProgSem.st{1}.`StP3 /\
+           Source.MultiPartyAPISemantics.ib Source.ProgSem.st{2} = Target.ProgSem.st{1}.`ib /\
+           Source.MultiPartyAPISemantics.ob Source.ProgSem.st{2} = Target.ProgSem.st{1}.`ob /\
+           Source.MultiPartyAPISemantics.StP1 Source.ProgSem.st{2} = Source.MultiPartyAPISemantics.StP2 Source.ProgSem.st{2} /\
+           Source.MultiPartyAPISemantics.StP2 Source.ProgSem.st{2} = Source.MultiPartyAPISemantics.StP3 Source.ProgSem.st{2}
            ==> _).
  rewrite /inv => |> *; auto.
  split; [|split; [|smt()]].
-  move: H11 => [??[?[??]]].
-  move: (bisim_backward2 _ _ _ _ H14 H15 _); first smt().
+  move: H10 => [??[?[??]]].
+  move: (bisim_backward2 _ _ _ _ H13 H14 _); first smt().
   move=> [??] [?[??]].
-  have ?:= (stepPiter_det _ _ _ _ _ _ _ _ H _ H16 _); first 4 smt().
-  by move: H16; rewrite -H19 H; move => /#.
- move: H12 => [??[?[??]]].
- move: (bisim_backward3 _ _ _ _ H14 H15 _); first smt().
+
+have ?: Source.MultiPartyAPISemantics.SemP1.stepPiter Source.MultiPartyAPISemantics.SemP1.stepL ks0
+        Source.ProgSem.st{2}.`Source.MultiPartyAPISemantics.StP1 = Some ss'0.
+rewrite -H15.
+cut ->: Source.MultiPartyAPISemantics.SemP1.stepL = Source.MultiPartyAPISemantics.SemP2.stepL.
+rewrite fun_ext /(==) => *.
+smt().
+rewrite H7.
+done.
+
+  have ?:= (Source.MultiPartyAPISemantics.SemP2.stepPiter_det _ _ _ _ _ _ _ _ H _ H18 _); first 4 smt().
+  by move: H18; rewrite -H19 H; move => /#.
+ move: H11 => [??[?[??]]].
+ move: (bisim_backward3 _ _ _ _ H13 H14 _); first smt().
  move=> [??] [?[??]].
- have ?:= (stepPiter_det _ _ _ _ _ _ _ _ H _ H16 _); first 4 smt().
- by move: H16; rewrite -H19 H; move => /#.
-seq 0 3: (ss' = (oget ProgSem.st{2}.`Sigma.[1]) /\
+
+have ?: Source.MultiPartyAPISemantics.SemP1.stepPiter Source.MultiPartyAPISemantics.SemP1.stepL ks0
+        Source.ProgSem.st{2}.`Source.MultiPartyAPISemantics.StP1 = Some ss'0.
+rewrite -H15.
+cut ->: Source.MultiPartyAPISemantics.SemP1.stepL = Source.MultiPartyAPISemantics.SemP3.stepL.
+rewrite fun_ext /(==) => *.
+smt().
+rewrite H7 H8.
+done.
+
+ have ?:= (Source.MultiPartyAPISemantics.SemP3.stepPiter_det _ _ _ _ _ _ _ _ H _ H18 _); first 4 smt().
+ by move: H18; rewrite -H19 H; move => /#.
+
+seq 0 3: (ss' = Source.ProgSem.st{2}.`Source.MultiPartyAPISemantics.StP1 /\
           #[/3:]pre).          
  sp 0 2.
  while {2} ((b = (i <= ks)){2} /\
              0 <= i{2} <= ks+1 /\ 
-             (stepPiter stepL ks ss = Some ss') /\
-             (stepPiter stepL (i+b2i b-1) ss = ProgSem.st{2}.`Sigma.[1]){2} /\
+             (Source.MultiPartyAPISemantics.SemP1.stepPiter Source.MultiPartyAPISemantics.SemP1.stepL ks ss = Some ss') /\
+             (oget (Source.MultiPartyAPISemantics.SemP1.stepPiter Source.MultiPartyAPISemantics.SemP1.stepL (i+b2i b-1) ss) = Source.ProgSem.st{2}.`Source.MultiPartyAPISemantics.StP1){2} /\
              #[/5:]pre
             ) (ks+1-i{2}).
-   move=> *; exlim ProgSem.st => sw.
+   move=> *; exlim Source.ProgSem.st => sw.
    case (i = ks).
-    wp; call (stepP_spec 3 sw).
-    call (stepP_spec 2 sw). 
-    call (stepP_spec 1 sw).
+    wp; call (stepP_spec P3 sw).
+    call (stepP_spec P2 sw). 
+    call (stepP_spec P1 sw).
     skip=> *.
-    have Hloop: stepPiter stepL 1 (oget ProgSem.st{hr}.`Sigma.[1])
+    have Hloop: Source.MultiPartyAPISemantics.SemP1.stepPiter Source.MultiPartyAPISemantics.SemP1.stepL 1 (Source.ProgSem.st{hr}.`Source.MultiPartyAPISemantics.StP1)
                 = None.
      move: H; progress.
-     move: H2; rewrite H18 b2i1 /= H1 => <- /=.
-     by move: (callSt_stepPiter stepL 1 ss' _); smt().
+     move: H2; rewrite H17 b2i1 /= H1 => <- /=.
+     by move: (Source.MultiPartyAPISemantics.SemP1.callSt_stepPiter Source.MultiPartyAPISemantics.SemP1.stepL 1 ss' _); smt().
     move: H; rewrite /inv;
-    progress; 1..6,8..: smt(stepPiter0 get_set_id).
-    - rewrite !H17 Hloop b2i0 /=; smt(get_setE).
-   wp; call (stepP_spec 3 
+progress.
+smt(Source.MultiPartyAPISemantics.SemP1.stepPiter0 get_set_id).
+have ?: Source.MultiPartyAPISemantics.SemP1.stepPiter Source.MultiPartyAPISemantics.SemP1.stepL 1 Source.ProgSem.st{hr}.`StP1 = Source.MultiPartyAPISemantics.SemP2.stepPiter Source.MultiPartyAPISemantics.SemP2.stepL 1 Source.ProgSem.st{hr}.`StP2.
+cut ->: Source.MultiPartyAPISemantics.SemP2.stepL = Source.MultiPartyAPISemantics.SemP1.stepL.
+smt(-local_source_step12).
+rewrite H15.
+rewrite /stepPiter.
+congr.
+have hloop2 : Source.MultiPartyAPISemantics.SemP2.stepPiter Source.MultiPartyAPISemantics.SemP2.stepL 1 Source.ProgSem.st{hr}.`StP2 = None.
+smt().
+rewrite hloop2.
+rewrite /b2i /=.
+smt(Source.MultiPartyAPISemantics.SemP2.stepPiter0 get_set_id).
+have ?: Source.MultiPartyAPISemantics.SemP1.stepPiter Source.MultiPartyAPISemantics.SemP1.stepL 1 Source.ProgSem.st{hr}.`StP1 = Source.MultiPartyAPISemantics.SemP3.stepPiter Source.MultiPartyAPISemantics.SemP3.stepL 1 Source.ProgSem.st{hr}.`StP3.
+cut ->: Source.MultiPartyAPISemantics.SemP3.stepL = Source.MultiPartyAPISemantics.SemP1.stepL.
+smt().
+rewrite H15 H16.
+rewrite /stepPiter.
+congr.
+have hloop3 : Source.MultiPartyAPISemantics.SemP3.stepPiter Source.MultiPartyAPISemantics.SemP3.stepL 1 Source.ProgSem.st{hr}.`StP3 = None.
+smt().
+rewrite hloop3.
+rewrite /b2i /=.
+smt(Source.MultiPartyAPISemantics.SemP3.stepPiter0 get_set_id).
+smt().
+have ?: Source.MultiPartyAPISemantics.SemP1.stepPiter Source.MultiPartyAPISemantics.SemP1.stepL 1 Source.ProgSem.st{hr}.`StP1 = Source.MultiPartyAPISemantics.SemP3.stepPiter Source.MultiPartyAPISemantics.SemP3.stepL 1 Source.ProgSem.st{hr}.`StP3.
+cut ->: Source.MultiPartyAPISemantics.SemP3.stepL = Source.MultiPartyAPISemantics.SemP1.stepL.
+smt().
+rewrite H15 H16.
+rewrite /stepPiter.
+congr.
+have hloop3 : Source.MultiPartyAPISemantics.SemP3.stepPiter Source.MultiPartyAPISemantics.SemP3.stepL 1 Source.ProgSem.st{hr}.`StP3 = None.
+smt().
+rewrite hloop3.
+rewrite /b2i /=.
+smt(Source.MultiPartyAPISemantics.SemP3.stepPiter0 get_set_id).
+have ?: Source.MultiPartyAPISemantics.SemP1.stepPiter Source.MultiPartyAPISemantics.SemP1.stepL 1 Source.ProgSem.st{hr}.`StP1 = Source.MultiPartyAPISemantics.SemP3.stepPiter Source.MultiPartyAPISemantics.SemP3.stepL 1 Source.ProgSem.st{hr}.`StP3.
+cut ->: Source.MultiPartyAPISemantics.SemP3.stepL = Source.MultiPartyAPISemantics.SemP1.stepL.
+smt().
+rewrite H15 H16.
+rewrite /stepPiter.
+congr.
+have hloop3 : Source.MultiPartyAPISemantics.SemP3.stepPiter Source.MultiPartyAPISemantics.SemP3.stepL 1 Source.ProgSem.st{hr}.`StP3 = None.
+smt().
+rewrite hloop3.
+rewrite /b2i /=.
+smt(Source.MultiPartyAPISemantics.SemP3.stepPiter0 get_set_id).
+smt().
+   wp; call (stepP_spec P3 
     {| sw with Sigma = sw.`Sigma.[
         1 <- oget (stepPiter stepL 1 (oget (sw.`Sigma.[1])))].[
         2 <- oget (stepPiter stepL 1 (oget (sw.`Sigma.[1])))] |}).
@@ -720,660 +841,3 @@ qed.
 
 end section MTSecurityProof.
 
-
-
-
-
-
-
-
-
-
-
-
-
-
-
-
-
-
-
-
-
-
-
-end Compilation.
-
-
-
-theory MultiThreaded.
-
-clone import SingleThreaded as ST with op n_parties <- 3, op n_corrupted <- 3.
-
-(* Target Languages *)
-
-(* Programs *)
-type L1.
-type L2.
-type L3.
-
-(* Environment *)
-type EnvL1.
-type EnvL2.
-type EnvL3.
-
-(* initial state *)
-op initStateL1 (P:L1): L1*EnvL1.
-op initStateL2 (P:L2): L2*EnvL2.
-op initStateL3 (P:L3): L3*EnvL3.
-
-type StateL1 = (L1, EnvL1) APIst.
-type StateL2 = (L2, EnvL2) APIst.
-type StateL3 = (L3, EnvL3) APIst.
-
-(* (local) Step semantics *)
-op stepL1 : L1 -> EnvL1 -> apiRes_data option -> ((L1,EnvL1) ECall) option.
-op stepL2 : L2 -> EnvL2 -> apiRes_data option -> ((L2,EnvL2) ECall) option.
-op stepL3 : L3 -> EnvL3 -> apiRes_data option -> ((L3,EnvL3) ECall) option.
-
-
-(* ASSUMPTION: backward simulation (trace preservation) *)
-axiom bisim_backward1 ss st kt st':
- equivSt ss st =>
- stepPiter stepL1 kt st = Some st' =>
- callSt st' <> None =>
- (exists ks ss', stepPiter stepL ks ss = Some ss'
-                 /\ equivSt ss' st' /\ 0 <= ks).
-
-axiom bisim_backward2 ss st kt st':
- equivSt ss st =>
- stepPiter stepL2 kt st = Some st' =>
- callSt st' <> None =>
- (exists ks ss', stepPiter stepL ks ss = Some ss'
-                 /\ equivSt ss' st' /\ 0 <= ks).
-
-axiom bisim_backward3 ss st kt st':
- equivSt ss st =>
- stepPiter stepL3 kt st = Some st' =>
- callSt st' <> None =>
- (exists ks ss', stepPiter stepL ks ss = Some ss'
-                 /\ equivSt ss' st' /\ 0 <= ks).
-
-
-
-(* handling different paces among parties *)
-op advSt ['l,'e] step (ss: (L,EnvL) APIst) (st: ('l,'e) APIst) : bool =
- exists n st', 0 <= n /\ equivSt ss st' /\ stepPiter step n st' = Some st.
-
-lemma advSt0 ['l, 'e] step s1 (s2: ('l, 'e) APIst):
- equivSt s1 s2 => advSt step s1 s2.
-proof.
-move=> *; exists 0 s2; progress.
-by rewrite stepPiter0.
-qed.
-
-lemma nosmt advSt_callSt ['l, 'e] step s1 (s2: ('l, 'e) APIst):
- advSt step s1 s2 =>
- callSt s1 <> None =>
- equivSt s1 s2.
-proof.
-move=> [k st'] /> *.
-have ?: callSt st' <> None by smt().
-move: (callSt_stepPiter step k st' H4); move=> [?|?].
- by move: H2; rewrite stepPiter0 //.
-by move: H2; rewrite H5.
-qed.
-
-
-
-(* END languages *)
-
-
-
-
-(* Global state for the multi-target setting (every party uses the same language) *)
-type GlobalMTSt = { P1: StateL1
-                  ; P2: StateL2
-                  ; P3: StateL3
-                  ; ibmt: sharedValue_t option
-                  ; obmt: sharedValue_t option
-                  }.
-
-
-
-
-(* updates a local state after a [stepP] *)
-op upd_P1 (newst: (L1,EnvL1) ECall) (st: GlobalMTSt): GlobalMTSt=
- {| st with P1 = st_from_step newst |}.
-op upd_P2 (newst: (L2,EnvL2) ECall) (st: GlobalMTSt): GlobalMTSt=
- {| st with P2 = st_from_step newst |}.
-op upd_P3 (newst: (L3,EnvL3) ECall) (st: GlobalMTSt): GlobalMTSt=
- {| st with P3 = st_from_step newst |}.
-(* updates all local states after a [stepS] *)
-op upd_P_API (r: apiRes_data option) (st: GlobalMTSt): GlobalMTSt =
- {| st with P1 = updRes r (P1 st); P2 = updRes r (P2 st); P3 = updRes r (P3 st) |}.
-(* updates the input buffer *)
-op upd_ibmt (newib: sharedValue_t option) (st: GlobalMTSt): GlobalMTSt =
- {| st with ibmt = newib |}.
-(* updates the output buffer *)
-op upd_obmt (newob: sharedValue_t option) (st: GlobalMTSt): GlobalMTSt =
- {| st with obmt = newob |}.
-
-
-(* initial [GlobalMTSt] *)
-op init_GlobalMTSt (P: L) : GlobalMTSt =
- {| P1 = iniSt (initStateL1 (compiler1 P))
-  ; P2 = iniSt (initStateL2 (compiler2 P))
-  ; P3 = iniSt (initStateL3 (compiler3 P))
-  ; ibmt = None
-  ; obmt = None
- |}.
-
-module ProgSemMT (API: API_t) = {
-  var st: GlobalMTSt
-  proc init(P: L): unit = {
-    API.api_init();
-    st <- init_GlobalMTSt P;
-  }
-  (* Step Public *)
-  proc stepP(id: partyId_t): bool = {
-    var r <- false;
-    var newst1 <- stepL1 (progSt (P1 st)) (envSt (P1 st)) (resSt (P1 st));
-    var newst2 <- stepL2 (progSt (P2 st)) (envSt (P2 st)) (resSt (P2 st));
-    var newst3 <- stepL3 (progSt (P3 st)) (envSt (P3 st)) (resSt (P3 st));
-    if (id = 1 && callSt (P1 st) = None && newst1 <> None) {
-      r <- true;
-      st <- upd_P1 (oget newst1) st;
-    }
-    if (id = 2 && callSt (P2 st) = None && newst2 <> None) {
-      r <- true;
-      st <- upd_P2 (oget newst2) st;
-    }
-    if (id = 3 && callSt (P3 st) = None && newst3 <> None) {
-      r <- true;
-      st <- upd_P3 (oget newst3) st;
-    }
-    return r;
-  }
-  (* Step Secret *)
-  proc stepS(): sideInfo_t option = {
-    var x, v, t;
-    var r <- None;
-    var ecall <- syncPoint [callSt (P1 st); callSt (P2 st); callSt (P3 st)];
-    if (ecall <> None) { (* call to the API *)
-      match (oget ecall) with
-      | Call_declass a => { (v, t) <@ API.api_declass(a);
-                            r <- Some t;
-                            (* updates API result *)
-                            st <- upd_P_API (Some v) st;
-                          }
-      | Call_in a => { if (ibmt st <> None) {
-                         t <@ API.api_in(a, oget (ibmt st));
-                         r <- Some t;
-                         st <- upd_ibmt None st; (* clears buffer *)
-                         st <- upd_P_API None st; (* resets call *)
-                       }
-                     }
-      | Call_out a => { if (obmt st = None) {
-                          (x, t) <@ API.api_out(a);
-                          r <- Some t;
-                          st <- upd_obmt (Some x) st; (* fills buffer *)
-                          st <- upd_P_API None st; (* resets call *)
-                          }
-                      }
-      | Call_sop o a pargs sargs => { t <@ API.api_sop(o, pargs, sargs, a);
-                                      r <- Some t;
-                                      st <- upd_P_API None st; (* resets call *)
-                                    }
-      end;
-    }
-    return r;
-  }
-  proc setInput(x: sharedValue_t): bool = {
-    var r <- false;
-    if (ibmt st = None) {
-      r <- true;
-      st <- upd_ibmt (Some x) st;
-    }
-    return r;
-  }
-  proc getOutput(): sharedValue_t option = {
-    var r: sharedValue_t option;
-    r <- obmt st;
-    if (r <> None) {
-      st <- upd_obmt None st;
-    }
-    return r;
-  }
-}.
-
-
-
-module RealSemMT: RealSemInterface = {
-  module PSem = ProgSemMT(API_Real)
-  include PSem
-}.
-
-module AdvOrclMT (Sem: AdvSemInterface) : AdvSemInterface = {
-  (* Simulator runs a local copy of all parties... *)
-  module SemEmu = RealSemMT
-  include SemEmu [- init, stepP, stepS]
-
-  proc init(P:L): unit = {
-    SemEmu.init(P);
-  }
-  (* [stepP] relies on the local [RealSemMT] module in order to
-     control the execution of each party.
-     It leaves [Sem] untouched *)
-  proc stepP = SemEmu.stepP
-  (* Step Secret *)
-  proc stepS(): sideInfo_t option = {
-    var b, i, v;
-    var r <- None;
-    var ecall <- syncPoint [callSt (P1 SemEmu.PSem.st);
-                            callSt (P2 SemEmu.PSem.st);
-                            callSt (P3 SemEmu.PSem.st)];
-    if (ecall <> None) { (* call to the API *)
-      (* advance the source into a sync-point *)
-      i <- 0;
-      b <- true;
-      while (b) {
-        b <@  Sem.stepP(1);
-        b <@  Sem.stepP(2);
-        b <@  Sem.stepP(3);
-        i <- i + 1;
-      }
-      (* do a [stepS] at the source *)
-      r <@ Sem.stepS();
-      if (r <> None) {
-          match (oget ecall) with
-          | Call_declass a => { v <- leakage_value (oget (oget r).`leakage);
-                                (* updates API result *)
-                                RealSemMT.PSem.st <- upd_P_API (Some (oget v)) RealSemMT.PSem.st;
-                              }
-          | Call_in a => { RealSemMT.PSem.st <- upd_P_API None RealSemMT.PSem.st; (* resets call *)
-                         }
-          | Call_out a => { RealSemMT.PSem.st <- upd_P_API None RealSemMT.PSem.st; (* resets call *)
-                          }
-      | Call_sop o a pargs sargs => { RealSemMT.PSem.st <- upd_P_API None RealSemMT.PSem.st; (* resets call *)
-                                    }
-      end;
-      }        
-    }
-    return r;
-  }
-}.
-
-module AdvMT (A: AdvInterface) (S:AdvSemInterface) : AdvEnvInterface = {
-  module AdvO = AdvOrclMT(S)
-  module Adv = A(AdvO)
-  proc init(P: L): unit = {
-    AdvO.init(P);
-    Adv.init(P);
-  }
-  proc activate = Adv.activate
-}.
-
-module REAL_MT (E: Env) (A: AdvInterface) = {
-  module Sem = RealSemMT
-  module Adv = A(Sem)
-  module Z = E(EnvO(Sem, Adv))
-  proc game(P: L): bool = {
-    var b;
-    Sem.init(P);
-    Adv.init(P);
-    b <@ Z.animate();
-    return b;
-  }
-}.
-
-
-section MTSecurityProof.
-
-declare module A: AdvInterface{ProgSem, ProgSemMT, AdvOrclMT}.
-declare module Z: Env{A, API_Real, ProgSem, ProgSemMT, AdvOrclMT}.
-
-op inv (stMT1 stMT2: GlobalMTSt) (stST2: GlobalSt) =
- stMT2.`P1 = stMT1.`P1 /\
- stMT2.`P2 = stMT1.`P2 /\
- stMT2.`P3 = stMT1.`P3 /\
- stST2.`ib = stMT1.`ibmt /\
- stST2.`ob = stMT1.`obmt /\
- stST2.`Sigma.[1] <> None /\
- stST2.`Sigma.[2] = stST2.`Sigma.[1] /\
- stST2.`Sigma.[3] = stST2.`Sigma.[1] /\
- advSt stepL1 (oget stST2.`Sigma.[1]) stMT1.`P1 /\
- advSt stepL2 (oget stST2.`Sigma.[1]) stMT1.`P2 /\
- advSt stepL3 (oget stST2.`Sigma.[1]) stMT1.`P3.
-
-local lemma nosmt stepP_prop:
- equiv [ RealSemMT.stepP ~ AdvOrclMT(RealSem).stepP:
-         ={id} /\ ={API_Real.senv} /\
-         inv ProgSemMT.st{1} ProgSemMT.st{2} ProgSem.st{2}
-         ==>
-         ={res} /\ ={API_Real.senv} /\
-         inv ProgSemMT.st{1} ProgSemMT.st{2} ProgSem.st{2} ].
-proof.
-proc; wp; skip; rewrite /inv; progress.
-- smt(). smt(). smt(). smt(). smt(). smt(). smt(). smt().
-- move: H7 => [??[?[??]]].
-  exists (n+1) st'; progress; rewrite /upd_P1 /=; first smt().
-  apply: (stepPiterS_some _ _ _ _ _ _ H15) => //=.
-  by rewrite -some_oget //.
-- smt(). smt(). smt(). smt(). smt(). smt(). smt(). smt().
-  smt(). smt(). smt().
-- move: H8 => [??[?[??]]].
-  exists (n+1) st'; progress; rewrite /upd_P2 /=; first smt().
-  apply: (stepPiterS_some _ _ _ _ _ _ H16) => //=.
-  by rewrite -some_oget //.
-- smt(). smt(). smt(). smt(). smt(). smt(). smt(). smt().
-  smt(). smt(). smt().
-- move: H9 => [??[?[??]]].
-  exists (n+1) st'; progress; rewrite /upd_P3 /=; first smt().
-  apply: (stepPiterS_some _ _ _ _ _ _ H17) => //=.
-  by rewrite -some_oget //.
-- smt(). smt(). smt().
-qed.
-
-local lemma nosmt stepS_prop:
- equiv [ RealSemMT.stepS ~ AdvOrclMT(RealSem).stepS:
-         true /\ ={API_Real.senv} /\
-         inv ProgSemMT.st{1} ProgSemMT.st{2} ProgSem.st{2}
-         ==>
-         ={res} /\ ={API_Real.senv} /\
-         inv ProgSemMT.st{1} ProgSemMT.st{2} ProgSem.st{2} ].
-proof.
-proc.
-sp 2 2; simplify.
-if; [smt() | | by skip; progress].
-seq 0 0: ((exists ks ss',
-            stepPiter stepL ks (oget ProgSem.st{2}.`Sigma.[1])
-            = Some ss' /\
-            equivSt ss' ProgSemMT.st{1}.`P1 /\ 0 <= ks)
-          /\ #[/:]pre).
- skip; rewrite /inv => |> *.
- move: H7 => [??[?[??]]].
- apply (bisim_backward1 _ _ _ _ H11 H12 _); smt(). 
-elim* => ??.
-exists* (oget ProgSem.st{2}.`Sigma.[1]); elim* => ss.
-conseq (_: ss = oget ProgSem.st{2}.`Sigma.[1] /\
-           stepPiter stepL ks ss = Some ss' /\
-           equivSt ss' ProgSemMT.st{1}.`P1 /\
-           equivSt ss' ProgSemMT.st{1}.`P2 /\
-           equivSt ss' ProgSemMT.st{1}.`P3 /\
-           ={r,ecall,API_Real.senv} /\
-           0 <= ks /\ r{2}=None /\
-           ecall{2} = callSt ProgSemMT.st{2}.`P1 /\
-           ecall{2} = callSt ProgSemMT.st{2}.`P2 /\
-           ecall{2} = callSt ProgSemMT.st{2}.`P3 /\
-           ecall{2} <> None /\
-           ProgSemMT.st{2}.`P1 = ProgSemMT.st{1}.`P1 /\
-           ProgSemMT.st{2}.`P2 = ProgSemMT.st{1}.`P2 /\
-           ProgSemMT.st{2}.`P3 = ProgSemMT.st{1}.`P3 /\
-           ProgSem.st{2}.`ib = ProgSemMT.st{1}.`ibmt /\
-           ProgSem.st{2}.`ob = ProgSemMT.st{1}.`obmt /\
-           ProgSem.st{2}.`Sigma.[1] <> None /\
-           ProgSem.st{2}.`Sigma.[2] = ProgSem.st{2}.`Sigma.[1] /\
-           ProgSem.st{2}.`Sigma.[3] = ProgSem.st{2}.`Sigma.[1]
-           ==> _).
- rewrite /inv => |> *; auto.
- split; [|split; [|smt()]].
-  move: H11 => [??[?[??]]].
-  move: (bisim_backward2 _ _ _ _ H14 H15 _); first smt().
-  move=> [??] [?[??]].
-  have ?:= (stepPiter_det _ _ _ _ _ _ _ _ H _ H16 _); first 4 smt().
-  by move: H16; rewrite -H19 H; move => /#.
- move: H12 => [??[?[??]]].
- move: (bisim_backward3 _ _ _ _ H14 H15 _); first smt().
- move=> [??] [?[??]].
- have ?:= (stepPiter_det _ _ _ _ _ _ _ _ H _ H16 _); first 4 smt().
- by move: H16; rewrite -H19 H; move => /#.
-seq 0 3: (ss' = (oget ProgSem.st{2}.`Sigma.[1]) /\
-          #[/3:]pre).          
- sp 0 2.
- while {2} ((b = (i <= ks)){2} /\
-             0 <= i{2} <= ks+1 /\ 
-             (stepPiter stepL ks ss = Some ss') /\
-             (stepPiter stepL (i+b2i b-1) ss = ProgSem.st{2}.`Sigma.[1]){2} /\
-             #[/5:]pre
-            ) (ks+1-i{2}).
-   move=> *; exlim ProgSem.st => sw.
-   case (i = ks).
-    wp; call (stepP_spec 3 sw).
-    call (stepP_spec 2 sw). 
-    call (stepP_spec 1 sw).
-    skip=> *.
-    have Hloop: stepPiter stepL 1 (oget ProgSem.st{hr}.`Sigma.[1])
-                = None.
-     move: H; progress.
-     move: H2; rewrite H18 b2i1 /= H1 => <- /=.
-     by move: (callSt_stepPiter stepL 1 ss' _); smt().
-    move: H; rewrite /inv;
-    progress; 1..6,8..: smt(stepPiter0 get_set_id).
-    - rewrite !H17 Hloop b2i0 /=; smt(get_setE).
-   wp; call (stepP_spec 3 
-    {| sw with Sigma = sw.`Sigma.[
-        1 <- oget (stepPiter stepL 1 (oget (sw.`Sigma.[1])))].[
-        2 <- oget (stepPiter stepL 1 (oget (sw.`Sigma.[1])))] |}).
-   call (stepP_spec 2 {| sw with Sigma = sw.`Sigma.[
-        1 <- oget (stepPiter stepL 1 (oget (sw.`Sigma.[1])))] |}). 
-   call (stepP_spec 1 sw).
-   skip => *.
-   have Hloop: stepPiter stepL 1 (oget ProgSem.st{hr}.`Sigma.[1])
-               <> None.
-    apply (stepPiter_lt _ ks i{hr} ss); first 2 smt().
-    rewrite -some_oget 1:/#.
-    move: H; progress; smt().
-   move: H; rewrite /inv; progress; 1..7,9..12: smt(get_setE).
-   - rewrite !get_setE /=.
-     rewrite H17 Hloop b2i1 /= -some_oget //.
-     rewrite stepPiterS; first smt().
-     move: H2; rewrite H18 b2i1 /= => ->.
-     by rewrite (some_oget ProgSem.st{hr}.`Sigma.[1]) /#.
- skip; progress; 1..2,4..5: smt().
- by rewrite b2i1 /= stepPiter0 // -some_oget /#.
-inline RealSem.stepS.
-seq 0 2: (#[/:]pre /\ r0{2} = None /\ ecall{1}=ecall0{2}).
- wp; skip; rewrite /inv; progress.
- rewrite /allECalls (_:3 = 1+1+1) 1:// !iotaS // iota1 /=.
- by rewrite !H12 !H13 /= H3 (equivSt_callSt _ _ H) /#.
-rcondt {2} 1; first by move=>*; skip; progress.
-match; move=> *. 
-- (* call_declass *)
-  split; move => [a Ha]; exists a; smt().
-- (* call_in *)
-  split; move => [a Ha]; exists a; smt().
-- (* call_out *)
-  split; move => [a Ha]; exists a; smt().
-- (* call_sop *)
-  split; move => [o a pargs sargs Ho]; exists o a pargs sargs; smt().
-- (* call_declass *)
-  inline API_Real.api_declass.
-  rcondt {2} 7.
-   move=> *; inline*; wp; rnd; wp; skip; progress; smt().
-  inline*; sp.
-  seq 1 1: (#pre /\ ={t0}); first by rnd; skip; progress; smt().
-  sp; match {2}.
-  + move=> *; wp; skip; progress; first 5 smt().
-    - by rewrite /upd_SigmaAPI /= mapE /= /updRes /upd_ib /=
-                 (some_oget st_R.`Sigma.[1]) // /#.
-    - by rewrite /upd_SigmaAPI /upd_ib /= !mapE /= /#.
-    - by rewrite /upd_SigmaAPI /upd_ib /= !mapE /= /#.
-    - exists 0 (upd_P_API (Some (oget (leakage_value (oget t0{2}.`leakage)))) st_L).`P1.
-      split; first done.
-      split; last by apply stepPiter0.
-      by rewrite /equivSt /upd_P_API /upd_SigmaAPI
-                 /= mapE /= /updRes /= oget_omap_some /#.
-    - exists 0 (upd_P_API (Some (oget (leakage_value (oget t0{2}.`leakage)))) st_L).`P2.
-      split; first done.
-      split; last by apply stepPiter0.
-      by rewrite /equivSt /upd_P_API /upd_SigmaAPI
-                 /= mapE /= /updRes /= oget_omap_some /#.
-    - exists 0 (upd_P_API (Some (oget (leakage_value (oget t0{2}.`leakage)))) st_L).`P3.
-      split; first done.
-      split; last by apply stepPiter0.
-      by rewrite /equivSt /upd_P_API /upd_SigmaAPI
-                 /= mapE /= /updRes /= oget_omap_some /#.
-  + move=> *; wp; skip; progress; smt().
-  + move=> *; wp; skip; progress; smt().
-  + move=> *; wp; skip; progress; smt().
-- (* call_in *)
-  if => //=; [smt() | |]; last first.
-   rcondf {2} 2; first by move=>*; wp; skip; progress.
-   by wp; skip; progress; smt(advSt0).
-  seq 1 1: (#pre /\ ={t}).
-   call (_: ={API_Real.senv} /\ a{1}=a0{2}).
-    by inline*; wp; rnd; wp; skip; progress.
-   by skip; progress; smt().
-  rcondt {2} 5; first by move=>*; wp; skip; progress.
-  sp; match {2}; move=> *.
-  + wp; skip; progress; smt().
-  + wp; skip; rewrite /inv => |>*; progress; first 3 smt().
-    - by rewrite /upd_SigmaAPI /= mapE /= /updRes /upd_ib /=
-                 (some_oget st_R.`Sigma.[1]) // /#.
-    - by rewrite /upd_SigmaAPI /upd_ib /= !mapE /= /#.
-    - by rewrite /upd_SigmaAPI /upd_ib /= !mapE /= /#.
-    - exists 0 (upd_P_API None (upd_ibmt None st_L)).`P1.
-      split; first done.
-      split; last by rewrite stepPiter0.
-      by rewrite /equivSt /upd_P_API /upd_ibmt /upd_SigmaAPI
-                 /= mapE /= /upd_ib /= /updRes /= get_some /#.
-    - exists 0 (upd_P_API None (upd_ibmt None st_L)).`P2.
-      split; first done.
-      split; last by rewrite stepPiter0.
-      by rewrite /equivSt /upd_P_API /upd_ibmt /upd_SigmaAPI
-                 /= mapE /= /upd_ib /= /updRes /= get_some /#.
-    - exists 0 (upd_P_API None (upd_ibmt None st_L)).`P3.
-      split; first done.
-      split; last by rewrite stepPiter0.
-      by rewrite /equivSt /upd_P_API /upd_ibmt /upd_SigmaAPI
-                 /= mapE /= /upd_ib /= /updRes /= get_some /#.
-  + wp; skip; progress; smt().
-  + wp; skip; progress; smt().
-- (* call_out *)
-  if => //=; [smt() | |]; last first.
-   rcondf {2} 2; first by move=>*; wp; skip; progress.
-   by wp; skip; progress; smt(advSt0).
-  seq 1 1: (#pre /\ ={x, t}).
-   call (_: ={API_Real.senv} /\ a{1}=a0{2}).
-    by inline*; wp; rnd; wp; skip; progress.
-   by skip; progress; smt().
-  rcondt {2} 5; first by move=>*; wp; skip; progress.
-  sp; match {2}; move=> *.
-  + wp; skip; progress; smt().
-  + wp; skip; progress; smt().
-  + wp; skip; rewrite /inv => |>*; progress; first 3 smt().
-    - by rewrite /upd_SigmaAPI /upd_P_API /upd_obmt /= mapE /#.
-    - by rewrite /upd_SigmaAPI /upd_ob /= !mapE /= /#.
-    - by rewrite /upd_SigmaAPI /upd_ob /= !mapE /= /#.
-    - exists 0 (upd_P_API None (upd_ibmt None st_L)).`P1.
-      split; first done.
-      split; last by rewrite stepPiter0.
-      by rewrite /equivSt /upd_P_API /upd_ibmt /upd_SigmaAPI
-                 /= mapE /= /upd_ib /= /updRes /= get_some /#.
-    - exists 0 (upd_P_API None (upd_ibmt None st_L)).`P2.
-      split; first done.
-      split; last by rewrite stepPiter0.
-      by rewrite /equivSt /upd_P_API /upd_ibmt /upd_SigmaAPI
-                 /= mapE /= /upd_ib /= /updRes /= get_some /#.
-    - exists 0 (upd_P_API None (upd_ibmt None st_L)).`P3.
-      split; first done.
-      split; last by rewrite stepPiter0.
-      by rewrite /equivSt /upd_P_API /upd_ibmt /upd_SigmaAPI
-                 /= mapE /= /upd_ib /= /updRes /= get_some /#.
-  + wp; skip; progress; smt().
-- (* call_sop *)
-  seq 1 1: (#pre /\ ={t}).
-   call (_: ={API_Real.senv} /\
-            (o,pargs,sargs,a){1}=(o0,pargs0,sargs0,a0){2}).
-    by inline*; wp; rnd; wp; skip; progress.
-   by skip; progress; smt(advSt0).
-  rcondt {2} 4; first by move=>*; wp; skip; progress.
-  sp; match {2}; move=> *.
-  + wp; skip; progress; smt().
-  + wp; skip; progress; smt().
-  + wp; skip; progress; smt().
-  + wp; skip; rewrite /inv => |>*; progress; first 3 smt().
-    - rewrite /upd_SigmaAPI /= mapE /= /updRes /upd_ib /=
-              (some_oget st_R.`Sigma.[1]) // /#.
-    - by rewrite /upd_SigmaAPI /= !mapE /= /#.
-    - by rewrite /upd_SigmaAPI /= !mapE /= /#.
-    - exists 0 (upd_P_API None (upd_ibmt None st_L)).`P1.
-      split; first done.
-      split; last by rewrite stepPiter0.
-      by rewrite /equivSt /upd_P_API /upd_ibmt /upd_SigmaAPI
-                 /= mapE /= /upd_ib /= /updRes /= get_some /#.
-    - exists 0 (upd_P_API None (upd_ibmt None st_L)).`P2.
-      split; first done.
-      split; last by rewrite stepPiter0.
-      by rewrite /equivSt /upd_P_API /upd_ibmt /upd_SigmaAPI
-                 /= mapE /= /upd_ib /= /updRes /= get_some /#.
-    - exists 0 (upd_P_API None (upd_ibmt None st_L)).`P3.
-      split; first done.
-      split; last by rewrite stepPiter0.
-      by rewrite /equivSt /upd_P_API /upd_ibmt /upd_SigmaAPI
-                 /= mapE /= /upd_ib /= /updRes /= get_some /#.
-qed.
-
-
-equiv SecurityMT:
- REAL_MT(Z, A).game ~ REAL(Z, AdvMT(A)).game
- : ={P, glob A, glob Z} ==> ={res}.
-proof.
-proc.
-call (_: ={glob A, API_Real.senv} /\
-         inv ProgSemMT.st{1} ProgSemMT.st{2} ProgSem.st{2}
-     ). 
-- (* setInput *)
-  by proc; inline*; wp; skip; progress; smt().
-- (* getOutput *)
-  by proc; inline*; wp; skip; progress; smt().
-- (* activate *)
-  proc; call (_: ={API_Real.senv} /\
-                 inv ProgSemMT.st{1} ProgSemMT.st{2} ProgSem.st{2}
-             ).
-  + (* stepP *)
-    by apply stepP_prop.
-  + (* stepS *)
-    by apply stepS_prop.
-    by skip; progress. 
-- inline*; call (_: ={API_Real.senv} /\
-                    inv ProgSemMT.st{1} ProgSemMT.st{2} ProgSem.st{2}
-                ).
-  by apply stepP_prop.
- by apply stepS_prop.
-wp; skip => /> *; progress.
-- rewrite /init_GlobalSt /= (_:3=1+1+1) 1:// !iotaS //= iota1 /=;
-  smt(get_setE).
-- rewrite /init_GlobalSt /= (_:3=1+1+1) 1:// !iotaS //= iota1 /=;
-  smt(get_setE).
-- rewrite /init_GlobalSt /= (_:3=1+1+1) 1:// !iotaS //= iota1 /=;
-  smt(get_setE).
-- rewrite /advStT; exists 0 (init_GlobalMTSt P{2}).`P1.
-  split; first done.
-  split; last by rewrite stepPiter0.
-  have ?:= (equivSt_init1 P{2}).
-  rewrite /init_GlobalSt /=  (_:3=1+1+1) 1:// !iotaS //= iota1 /=.
-  by rewrite !get_setE /#.
-- rewrite /advStT; exists 0 (init_GlobalMTSt P{2}).`P2.
-  split; first done.
-  split; last by rewrite stepPiter0.
-  have ?:= (equivSt_init2 P{2}).
-  rewrite /init_GlobalSt /=  (_:3=1+1+1) 1:// !iotaS //= iota1 /=.
-  by rewrite !get_setE /#.
-- rewrite /advStT; exists 0 (init_GlobalMTSt P{2}).`P3.
-  split; first done.
-  split; last by rewrite stepPiter0.
-  have ?:= (equivSt_init3 P{2}).
-  rewrite /init_GlobalSt /=  (_:3=1+1+1) 1:// !iotaS //= iota1 /=.
-  by rewrite !get_setE /#.
-qed.
-
-end section MTSecurityProof.
-
-
-end MultiThreaded.
-
-(*
-print MultiThreaded.SecurityMT.
-*)
