src/SPAPISemantics.ec
@@ -106,11 +106,11 @@ theory SinglePartyAPISemantics.
     type sideInfo_t = sideInfo_t.
 
 (* multiple steps... *)
-op stepPiter ['l, 'e]
-  (step: 'l -> 'e -> apiRes_data option -> (('l,'e) ECall) option)
+op stepPiter
+  (step: L -> EnvL -> apiRes_data option -> ((L,EnvL) ECall) option)
   (k:int)
-  (st:('l,'e) APIst)
-  : ('l,'e) APIst option =
+  (st:(L,EnvL) APIst)
+  : (L,EnvL) APIst option =
   IntExtra.IterOp.iter k
     (fun ost => if ost <> None && callSt (oget ost) = None
               then let st = oget ost in 
@@ -118,14 +118,14 @@ op stepPiter ['l, 'e]
                    omap st_from_step ecall else None) (Some st).
 
 lemma stepPiter0
- (step : 'l -> 'e -> apiRes_data option -> (('l,'e) ECall) option) 
+ (step : L -> EnvL -> apiRes_data option -> ((L,EnvL) ECall) option) 
  (k : int)
- (st : ('l,'e) APIst) :
+ (st : (L,EnvL) APIst) :
  k <= 0 =>
  stepPiter step k st = Some st.
 proof. by move => ?; rewrite /stepPplus iter0. qed.
 
-lemma nosmt stepPiter1 ['l, 'e] step (st:('l,'e) APIst):
+lemma nosmt stepPiter1  step (st:(L,EnvL) APIst):
  callSt st = None =>
  stepPiter step 1 st
  = omap st_from_step (step (progSt st) (envSt st) (resSt st)).
@@ -134,7 +134,7 @@ rewrite /stepPplus /progSt /envSt /resSt.
 by rewrite iter1 /= => ->.
 qed.
 
-lemma nosmt stepPiterS_none ['l, 'e] step k (s:('l,'e) APIst):
+lemma nosmt stepPiterS_none  step k (s:(L,EnvL) APIst):
  stepPiter step k s = None =>
  stepPiter step (k+1) s = None.
 proof.
@@ -144,7 +144,7 @@ case: (0 <= k) => E.
 smt(iter0).
 qed.
 
-lemma nosmt stepPiterS_some ['l, 'e] step k (s s':('l,'e) APIst) x:
+lemma nosmt stepPiterS_some  step k (s s':(L,EnvL) APIst) x:
  0 <= k =>
  stepPiter step k s = Some s' =>
  callSt s' = None =>
@@ -156,7 +156,7 @@ rewrite IntExtra.IterOp.iterS //= => *.
 by rewrite /st_from_step  H0 /= H1 H2.
 qed.
 
-lemma nosmt stepPiterS ['l, 'e] step k (s : ('l,'e) APIst):
+lemma nosmt stepPiterS  step k (s : (L,EnvL) APIst):
  0 <= k =>
  stepPiter step (k+1) s = obind (stepPiter step 1) (stepPiter step k s).
 proof.
@@ -168,7 +168,7 @@ case: (stepPiter step 1 st') => //= st''.
 by rewrite iter1.
 qed.
 
-lemma nosmt stepPiter_lt ['l, 'e] step (k i:int) (s s': ('l,'e) APIst):
+lemma nosmt stepPiter_lt  step (k i:int) (s s': (L,EnvL) APIst):
  0 <= i < k =>
  stepPiter step k s <> None =>
  stepPiter step i s = Some s' =>
@@ -184,7 +184,7 @@ case: {2}a (eq_refl a) => [|a'] Ea //=; rewrite Ea //=.
 move=> *; apply IH; smt(). 
 qed.
 
-lemma callSt_stepPiter ['l, 'e] step k (s:('l,'e) APIst):
+lemma callSt_stepPiter  step k (s:(L,EnvL) APIst):
  callSt s <> None =>
  k <= 0 \/ stepPiter step k s = None.
 proof.
@@ -197,7 +197,7 @@ move=> n Hn [?|?].
 by right; rewrite stepPiterS_none.
 qed.
 
-lemma nosmt stepPiter_det ['l, 'e] step k1 k2 (s s1' s2': ('l,'e) APIst):
+lemma nosmt stepPiter_det  step k1 k2 (s s1' s2': (L,EnvL) APIst):
  0 <= k1 =>
  0 <= k2 =>
  stepPiter step k1 s = Some s1' =>
